src/Specific/Framework/Pipeline.v
@@ -1,0 +1,86 @@
+Require Import Crypto.Arithmetic.Core. Import B.
+Require Import Crypto.Arithmetic.PrimeFieldTheorems.
+Require Import Crypto.Compilers.Syntax.
+Require Import Crypto.Compilers.SmartMap.
+Require Import Crypto.Compilers.Tuple.
+Require Import Crypto.Compilers.ExprInversion.
+Require Import Crypto.Compilers.Z.Syntax.Util.
+Require Import Crypto.Compilers.Z.Syntax.
+Require Import Crypto.Specific.Framework.RawCurveParameters.
+Require Import Crypto.Specific.Framework.ArithmeticSynthesis.Base.
+Require Import Crypto.Specific.Framework.OutputType.
+Require Import Crypto.Util.Notations.
+Import CurveParameters.Notations.
+
+Local Coercion Z.to_nat : Z >-> nat.
+Local Notation interp_flat_type := (interp_flat_type interp_base_type).
+
+Section with_curve.
+  Context (curve : RawCurveParameters.CurveParameters).
+
+  Local Notation RT := (RT curve).
+  Local Notation rT := (rT curve).
+  Local Notation T' := (T' curve).
+  Local Notation encode := (encode curve).
+  Local Notation decode := (decode curve).
+
+  Record SynthesisPreOutput :=
+    {
+      zero : Expr RT;
+      one : Expr RT;
+      add : Expr (rT * rT -> rT); (* does not include carry *)
+      sub : Expr (rT * rT -> rT); (* does not include carry *)
+      mul : Expr (rT * rT -> rT); (* includes carry *)
+      square : Expr (rT -> rT); (* includes carry *)
+      opp : Expr (rT -> rT); (* does not include carry *)
+      carry : Expr (rT -> rT);
+      carry_add : Expr (rT * rT -> rT)
+      := (carry ∘ add)%expr;
+      carry_sub : Expr (rT * rT -> rT)
+      := (carry ∘ sub)%expr;
+      carry_opp : Expr (rT -> rT)
+      := (carry ∘ opp)%expr;
+
+      P : T' -> Prop;
+
+      encode_valid : forall v, P (Interp (encode v) tt);
+
+      zero_correct : zero = encode 0%F; (* which equality to use here? *)
+      one_correct : one = encode 1%F; (* which equality to use here? *)
+
+      opp_valid : forall x, P x -> P (Interp carry_opp x);
+      add_valid : forall x y, P x -> P y -> P (Interp carry_add (x, y));
+      sub_valid : forall x y, P x -> P y -> P (Interp carry_sub (x, y));
+      mul_valid : forall x y, P x -> P y -> P (Interp mul (x, y));
+      square_correct : forall x, P x -> Interp square x = Interp mul (x, x);
+    }.
+
+  Definition FinalizeOutput (v : SynthesisPreOutput) : SynthesisOutput curve.
+  Proof.
+    simple refine (let ring_goal : _ /\ _ /\ _ := _ in _); [ shelve.. | | ]; cycle 1.
+    simple refine {|
+             OutputType.zero := v.(zero);
+             OutputType.one := v.(one);
+             OutputType.add := v.(add);
+             OutputType.sub := v.(sub);
+             OutputType.mul := v.(mul);
+             OutputType.opp := v.(opp);
+             OutputType.carry := v.(carry);
+             OutputType.square := v.(square);
+
+             OutputType.zero_correct := v.(zero_correct);
+             OutputType.one_correct := v.(one_correct);
+             OutputType.encode_valid := v.(encode_valid);
+             OutputType.add_valid := v.(add_valid);
+             OutputType.sub_valid := v.(sub_valid);
+             OutputType.mul_valid := v.(mul_valid);
+             OutputType.opp_valid := v.(opp_valid);
+             OutputType.square_correct := v.(square_correct);
+
+             OutputType.ring := proj1 ring_goal;
+             OutputType.encode_homomorphism := proj1 (proj2 ring_goal);
+             OutputType.decode_homomorphism := proj2 (proj2 ring_goal);
+           |}.
+    { intro x; cbv [decode encode Interp interp].
+      SearchAbout interpf SmartPairf.
+    constructor.
